

MAT439: Commutative Algebra

Mahmudul Hasan Turjoy

Last updated: February 11, 2026

Contents

1	Preface	1
2	Abstract Algebra Review (2/2/26)	1
2.1	Group Theory	1
2.2	Ring Theory	4
3	Ideals (09/02/26)	7
3.1	Quotient Ring	8
4	References	10

1 Preface

These lecture notes were taken in the course MAT439: Commutative Algebra, taught by Nian Ibne Nazrul at BRAC University, as part of the BSc in Mathematics program in Spring 2026. Each lecture corresponds to a chapter in these notes.

Nothing in these notes is original (except my mistakes); almost everything here can be found somewhere in [AM69] or [Eis95]. In particular, we adopt the notation of [AM69] for notational consistency.

If you find any mistake, please report it at mh.turjoy@yahoo.com, even if it is something very small, even if you are not sure.

2 Abstract Algebra Review (2/2/26)

This lecture provides a brief review of some of the materials covered in MAT311: Abstract Algebra, with motivations and detailed explanations in definitions and proofs omitted.

2.1 Group Theory

Definition 2.1 (Binary Operation)

Let S be a nonempty set. A *binary operation* on S is a map

$$* : S \times S \longrightarrow S.$$

We denote $*(x, y)$ by $x * y$.

Definition 2.2

Let $f : A \rightarrow B$ be a map and let $C \subseteq A$. The *restriction of f to C* is the map

$$f|_C : C \rightarrow B$$

defined by

$$f|_C(x) = f(x) \quad \text{for all } x \in C.$$

Definition 2.3 (Group)

A *group* is an ordered pair $(G, *)$, where G is a set and $*$ is a binary operation such that:

- **Associativity:** For all $g, h, k \in G$, $(g * h) * k = g * (h * k)$.
- **Identity element:** There exists an element $e \in G$ such that for all $g \in G$, $e * g = g = g * e$.
- **Inverse element:** For each $g \in G$, there exists an element $h \in G$ such that $g * h = e = h * g$.

If $(G, *)$ is a group, then we simply say G is a group, when what $*$ is, is clear from the context. G is called *abelian*¹ if $g * h = h * g$, for all $g, h \in G$.

Proposition 2.4

Let $(G, *)$ be a group. Then

- Identity element e is unique.
- Inverse h of an element $g \in G$ is unique. So we denote $h =: g^{-1}$.

After proving these results, we can use definite article “the” before identity element and inverse of a group element.

Proof. • Suppose there are two identity elements e_1, e_2 . Then

$$e_1 = e_1 * e_2 = e_2.$$

- Let $g \in G$ and suppose h, k are two inverses of g . Then

$$h = h * e = h * (g * k) = (h * g) * k = e * k = k.$$

□

Definition 2.5 (Subgroup)

Let S be a subset of a group $(G, *)$, and $*|_{S \times S} : S \times S \rightarrow G$ be the restriction of the map $*$. S is called a *subgroup* of G and denoted by $S \leq G$ if

- $e \in S$,
- For all $s \in S$, $s^{-1} \in S$,
- $\text{Im}(*|_{S \times S}) \subseteq S$.

In other words, if $(S, *|_{S \times S})$ is a group by itself.

One of the philosophies in mathematics in general is: to understand an object, you should study functions from that object. Following definition is important in that sense.

¹Some people capitalize the letter “A” in honor of mathematician Niels Henrik Abel, who contributed enormously in the subject.

Definition 2.6 (Group Homomorphism)

A map between groups $f : (G, *) \rightarrow (H, \#)$ is called a *group homomorphism* if

$$f(g * h) = f(g) \# f(h) \quad \forall g, h \in G.$$

The set

$$\ker f := f^{-1}(\{e\}),$$

is called the *kernel* of f .

Proposition 2.7

$\ker f \leq G$.

Proof. We verify three conditions of a subring:

1.

$$\begin{aligned} f(e_G) &= f(e_G * e_G) = f(e_G) \# f(e_G) \\ \implies f(e_G) \# (f(e_G))^{-1} &= (f(e_G) \# f(e_G)) \# (f(e_G))^{-1} \\ \implies f(e_G) \# (f(e_G))^{-1} &= f(e_G) \# (f(e_G) \# (f(e_G))^{-1}) \\ \implies e_G &= f(e_G) \\ \therefore e_G &\in \ker f. \end{aligned}$$

2. Let $s \in \ker f$, then $f(s) = e_H$. Then

$$\begin{aligned} f(s * s^{-1}) &= f(e_G) = e_H \\ \implies f(s) \# f(s^{-1}) &= e_H \\ \implies e_H \# f(s^{-1}) &= e_H \\ \implies f(s^{-1}) &= e_H \\ \therefore s^{-1} &\in \ker f. \end{aligned}$$

3. Let $K = \ker f$ and $s \in \text{Im}(*|_{K \times K})$. Then there exists $(r, t) \in K \times K$ such that $r * t = s$. We have to prove $s \in K$.

$$f(s) = f(r * t) = f(r) \# f(t) = e_H \# e_H = e_H.$$

Therefore, $\text{Im}(*|_{K \times K}) \subseteq K$.

□

Proposition 2.8

For all $g \in G$, $g \ker f = \ker f g$.

Generalising kernel using this key property, we define the following:

Definition 2.9 (Normal Subgroup)

A subgroup N of a group G is called *normal* if $gN = Ng$ for all $g \in G$. We denote it by $N \trianglelefteq G$.

Definition 2.10 (Coset)

Let $H \leq (G, *)$. Then for an element $g \in G$, the set

$$gH := \{g * h : h \in H\},$$

is called a *left coset* of G . Similarly,

$$Hg := \{h * g : h \in H\},$$

is called a *right coset*.

Definition 2.11 (Quotient Group)

Let $N \trianglelefteq G$. Then

$$G/N := \{gN : g \in G\},$$

is a group with group operation \cdot given by

$$(gN) \cdot (hN) = (gh)N.$$

We call it a *quotient group*.

The map $\pi : G \rightarrow G/N$ given via $g \mapsto gN$ is a group homomorphism. It is called *quotient map*. Kernel of this map is N . Hence,

Theorem 2.12

Any normal subgroup N of a group G can be written as the kernel of some group homomorphism.

Theorem 2.13 (1st Isomorphism Theorem)

Let $f : G \rightarrow H$ be a group homomorphism. Then $G/\ker f$ is isomorphic to $\text{Im} f$ by the isomorphism given via $g\ker f \mapsto f(g)$.

2.2 Ring Theory

Definition 2.14 (Ring)

A *ring* is a datum $(R, +, \cdot)$, where R is a set and $+, \cdot$ are binary operations such that:

- $(R, +)$ is an abelian group (so R has an identity element^a denoted by 0).
- $(g \cdot h) \cdot j = g \cdot (h \cdot j), \forall g, h, j \in R$.
- $g \cdot (h + j) = g \cdot h + g \cdot j$ and $(h + j) \cdot g = h \cdot g + j \cdot g, \forall g, h, j \in R$.

^aWe call it additive identity in the context of rings.

If there exists an element $1 \in R$ such that for all $x \in R, x \cdot 1 = x = 1 \cdot x$, then 1 is called *multiplicative identity* and R is called a *ring with identity*. In this course, we are primarily interested in commutative² rings with identity. So, from now on, every ring in these notes is a commutative ring with identity unless stated otherwise.

Proposition 2.15

If additive and multiplicative identities of a ring R are equal, then R is the trivial ring, i.e., $R = \{0\}$.

Proof. Let $x \in R$, then

$$x = x \cdot 1 = x \cdot 0 = 0 \implies R = \{0\}.$$

□

²As the name of the course suggests XD

Definition 2.16 (Ring Homomorphism)

Suppose $(R_1, +_1, *_1)$ and $(R_2, +_2, *_2)$ are two rings. Then a map $f : (R_1, +_1, *_1) \rightarrow (R_2, +_2, *_2)$ is called a *ring homomorphism* if

- $f(a +_1 b) = f(a) +_2 f(b)$,
- $f(a *_1 b) = f(a) *_2 f(b)$,
- $f(1_{R_1}) = 1_{R_2}$.

Exercise 2.17

To show that the third condition of the ring homomorphism is independent of the other two, find an example of a map between two rings that satisfies first two conditions, but not the third one.

Answer (Instructor). An example that satisfies the conditions $f(a + b) = f(a) + f(b)$ and $f(ab) = f(a)f(b)$ but not $f(1) = 1$ is the map $f : (\mathbb{Z}, +, *) \rightarrow (\mathbb{Z}, +, *)$, $f(n) = 0$ for all n , i.e. the zero map. $f(a + b) = 0 = 0 + 0 = f(a) + f(b)$, $f(ab) = 0 = 0 \times 0 = f(a)f(b)$, but $f(1) = 0 \neq 1$.

Definition 2.18 (Subring)

Suppose $S \subseteq R$ where $(R, +, \cdot)$ is a ring. If $(S, +|_{S \times S}, \cdot|_{S \times S})$ is a ring by itself, then S is called a subring of R .

Definition 2.19 (Ideal)

An *ideal* I of a ring R is a subset of R and satisfies:

- I is a subgroup of $(R, +)$,
- Let $IR := \{i \cdot r : i \in I \text{ and } r \in R\}$. Then $IR \subset I$.

Example 2.20 (Principle Ideal)

Suppose $a \in R$. Then $(a) := \{a \cdot r : r \in R\}$ is an ideal, also called as *principle ideal* or ideal generated by a .^a

^aIt seemed like every non-trivial ideal should be of this form. But Ernest Kummer first discovered ideals that were not generated by a single element, which exploded the subject.

Example 2.21

$R = \mathbb{Z}$ has an infinite number of ideals, explicitly

$$I = (n) = n\mathbb{Z}, \quad \forall n \geq 0.$$

In fact, every ideal of \mathbb{Z} is of this form^a. For all $n \in \mathbb{Z}$, (n) is an ideal of \mathbb{Z} . We now prove the converse.

Let P be an ideal of \mathbb{Z} . If $P = \{0\}$, then $P = (0)$.

Assume $P \neq \{0\}$. Since $P \leq \mathbb{Z}$, there exists a positive integer in P . Let

$$n = \min\{k \in P \mid k > 0\}.$$

We claim that $P = (n)$. Since $n \in P$ and P is an ideal, for any $z \in \mathbb{Z}$,

$$zn \in P,$$

hence $(n) \subseteq P$.

Conversely, let $p \in P$. By the Euclid's Division lemma, there exist $q, r \in \mathbb{Z}$ such that

$$p = qn + r, \quad 0 \leq r < n.$$

Since $p \in P$ and $qn \in P$, and P is an ideal, we have

$$r = p - qn \in P.$$

By the minimality of n , it follows that $r = 0$. Hence

$$p = qn \in (n),$$

and therefore $P \subseteq (n)$.

Thus,

$$P = (n).$$

^aIt is very rare that when you have a ring, you can list all of its ideals.

Example 2.22 (Polynomial Ring)

Let R be a ring, x be an indeterminate and define $R[x]$ be the set of all formal sums of the form

$$\sum a_i x^i = a_n x^n + a_{n-1} x^{n-1} + \cdots + a_1 x + a_0, \quad \text{where } \{i : a_i \neq 0\} \text{ is finite.}$$

Given two polynomials $f = \sum a_i x^i$ and $g = \sum b_i x^i$ in $R[x]$, the sum of f and g is defined as

$$f + g = \sum (a_i + b_i) x^i,$$

and the product of f and g as

$$f \cdot g = \sum c_i x^i, \quad \text{where } c_i = \sum_{j,k:j+k=i} a_j b_k.$$

With this rule of addition and multiplication, $(R[x], +, \cdot)$ becomes a ring, called *polynomial ring*.^a We can further define polynomial ring $R[x][y]$ over $R[x]$ and it turns out that $R[x][y] \cong R[x, y]$.^b Some of the ideals of the ring $R[x, y]$ are:

- $\langle x \rangle = \{xf(x, y) : f(x, y) \in R[x, y]\} = \{\text{All the polynomials with degree of } x \text{ at least } 1\}.$
- $\langle x, y \rangle = \{xf(x, y) + yg(x, y) : f, g \in R[x, y]\} = \{\text{All the polynomials with degree of no constant term}\}.$

^aIn the definition above, each $a_i \in R$ is called the coefficients of the polynomial; a_i is the coefficient of x^i and the zero element given as the polynomial with zero coefficients.

^bPolynomial ring of several indeterminates is not defined here though.

3 Ideals (09/02/26)

Proposition 3.1

Let \mathbb{K} be a field. Then every ideal of $\mathbb{K}[x]$ is principle, but it is not true in general in $\mathbb{K}[x_1, \dots, x_n]$ for $n > 1$.

Proof. We proceed similarly as in we did in the case of \mathbb{Z} . But before that, we have to prove analogous Euclid's Division lemma for $\mathbb{K}[x]$.

Claim 3.2. Let $f, g \in \mathbb{K}[x]$. If $g \neq 0$, then there exists polynomials $q, r \in \mathbb{K}[x]$ such $f = gq + r$, where $\deg r < \deg g$.

Proof of claim. If g divides f , then $r = 0$ and we are done. If not, let $r = f - gq$ be the polynomial of least degree among all polynomials of the form $f - lg$ with $l \in \mathbb{K}[x]$. Then we must have $\deg g > \deg r$. Otherwise, let the leading term of r and g be ax^m and bx^n respectively. Then

$$r - g \cdot ab^{-1}x^{m-n} = f - gq - g \cdot ab^{-1}x^{m-n} = f - g(q + ab^{-1}x^{m-n}),$$

has smaller degree than r and is of the given form, which contradicts minimality of the degree of r . \square

If $f \in \mathbb{K}[x]$, then (f) is an ideal. Conversely, if I is an ideal of $\mathbb{K}[x]$, we claim that $(g) = I$, where g is a polynomial of least positive degree in I . Clearly, $(g) \subseteq I$. Let $f \in I$, then by the **Claim 3.2**, there exists $q, r \in \mathbb{K}[x]$ such that

$$f = gq + r, \quad \text{where } \deg r < \deg g.$$

Here $r = 0$, otherwise, $r = f - gq \in I$, which contradicts the minimality of the degree of g . Hence, $f = gq \in (g)$, which implies $I \subseteq (g)$. Therefore, $I = (g)$.

However, in general, in $\mathbb{K}[x_1, \dots, x_n]$ for $n > 1$, every ideal is not principle. As counter-example, we can consider the finitely generated ideal (x_1, x_2) . \square

3.1 Quotient Ring

Definition 3.3 (Quotient Ring)

Suppose R is a (commutative) ring (with identity), and suppose I is an ideal of R . So, I is an additive subgroup of the abelian group $(R, +)$ ^a. R/I is a quotient group where elements look like $r + I$. Define multiplication on R/I :

$$(r + I) \cdot (r' + I) = rr' + I.$$

Then $(R/I, +, \cdot)$ becomes a ring called *quotient ring* of R modulo I .

^aFor an abelian group, every subgroup is normal, $r + H = H + r$.

Since cosets of an additive group $(R, +)$ can have multiple representatives, we have to check well-definedness of the multiplication defined above, i.e., if $r + I = h + I$ and $r' + I = h' + I$, then $(r + I) \cdot (r' + I) = (h + I) \cdot (h' + I)$. Notice, $r + I = h + I$ and $r' + I = h' + I \Leftrightarrow r - h \in I$ and $r' - h' \in I$. Since I is an ideal,

$$(r - h)r' \in I \implies rr' - hr' \in I \text{ and}$$

$$h(r' - h') \in I \implies hr' - hh' \in I.$$

Since I is an additive subgroup,

$$\begin{aligned} & (rr' - hr') + (hr' - hh') \in I \\ \implies & rr' + (-hr' + hr') - hh' \in I \\ \implies & rr' - hh' \in I \\ \implies & rr' + I = hh' + I \\ \therefore & (r + I) \cdot (r' + I) = (h + I) \cdot (h' + I). \end{aligned}$$

Associativity, distributive property, existence of identity (which is $0 + I = I$) and commutativity of $(R/I, +, \cdot)$ are routine checks.

Student Question

Can we take quotient modulo an ideal of a non-commutative ring?

Answer (Instructor). Yes, we can! In that case, the ideal should be two-sided ideal. Recall, in a non-commutative ring R , an additive subgroup I of R is called a left ideal if $RI \subseteq I$ and right ideal if $IR \subseteq I$. If I is both left and right ideal, then we call it a two-sided ideal. For example, **to be written....**

Proposition 3.4

Suppose R is a ring and I is an ideal. Then there is a 1 – 1 order-preserving correspondence between the ideals of R containing I and the ideals of the quotient ring R/I . The order-preserving 1 – 1 correspondence is given by: if J' is an ideal of R/I , then the corresponding ideal in R is given by $\pi^{-1}(J')$.^a

^a π is the canonical projection map that maps each element r of R to $r + I$ in R/I .

Proof. Step (1). First we show that if J' is an ideal of the quotient R/I , then $\pi^{-1}(J')$ is an ideal in R .

Firstly, $0 \in \pi^{-1}(J')$, because $\pi(0) = I \in J'$ as J' is an ideal of R/I , so it must contain the additive identity I of R/I .

Suppose $x, y \in \pi^{-1}(J')$. So $\pi(x) = x + I, \pi(y) = y + I \in J'$. Since J' is an ideal, we have

$$\begin{aligned} & (x + I) - (y + I) \in J' \\ \implies & (x - y) + I \in J' \\ \implies & \pi(x - y) \in J' \\ \implies & (x - y) \in \pi^{-1}(J'). \end{aligned}$$

Hence, using subgroup criterion, $\pi^{-1}(J')$ is an additive subgroup of R .

Also, if $r \in R$, then $r \cdot \pi^{-1}(J') \subseteq \pi^{-1}(J')$. To see that, suppose $x \in \pi^{-1}(J')$, which implies $x + I \in J'$, which implies $(r + I)(x + I) \in J'$ as $(r + I) \in R/I$, and that implies

$$rx + I \in J' \implies \pi(rx) \in J' \implies rx \in \pi^{-1}(J').$$

$\therefore \pi^{-1}(J')$ is indeed an ideal of R .

Step (2). We want to show that if J' is an ideal of R/I , then the ideal $J = \pi^{-1}(J')$ of R contains I .

Let $x \in I$, then $\pi(x) = I \in J'$, which implies $x \in \pi^{-1}(J')$. Therefore, $\ker \pi = I \subseteq \pi^{-1}(J')$.

Step (3). Lastly, we have to prove **to be written...**

□

Definition 3.5

Let R be a ring.

An element $r \in R$ is called a *zero-divisor* if there is a non-zero $y \in R$ such that $r \cdot y = 0$.

R is called an *integral domain* if it does not have any non-zero zero-divisors.

An element $r \in R$ is called *nilpotent* if $r^n = 0$ for some $n > 0$.

A *unit* $r \in R$ is an element that “divides 1” – i.e., for which there exists $y \in R, y \neq 0$ such that $xy = 1$.

R is a *field* if $1 \neq 0$ and every non-zero element is a unit.

Note 3.6 • 0 is also a zero-divisor.

- Nilpotent elements are all zero-divisors. To see that, suppose r is a nilpotent element and $r^n = 0$. If $n = 1$, then r is trivially zero-divisor. Otherwise, we have $r^{n-1} \in R$ such that $r \cdot r^{n-1} = 0$.
- The set of all units of a ring R forms an abelian group under multiplication and it is denoted by R^\times .
- A unit cannot be a zero-divisor in $R \neq (0)$. Suppose x is a unit with $xy = 1$. If x is also a zero-divisor, $sx = 0$ for some $s \neq 0$.

$$sx = 0 \implies (sx)y = 0y \implies s(xy) = 0 \implies s \cdot 1 = 0 \implies s = 0 \text{ (contradiction!)}$$

So,

- A field is an integral domain.

Proposition 3.7

Suppose R is a ring and $R \neq (0)$. Then the following are equivalent:

1. R is a field.
2. R only has two ideals: (0) and (1) .
3. Every homomorphism^a of R to a non-zero ring is injective.

^aRemember we require $f(1) = 1$ for a ring homomorphism f .

Proof. • (1) \implies (2). Suppose R is a field. That means, every non-zero element is a unit. Let I be an ideal of R . If $I = (0)$, we are done. Otherwise, there exists non-zero $x \in I \subseteq R$. Hence, x is a unit, i.e., there exists $y \in R$ such that $xy = yx = 1$. Since I is an ideal, $y \cdot x \in I \implies 1 \in I \implies I = (1) = R$.

- (2) \implies (3). Suppose R has only two ideals: (0) and (1) . And let $f : R \rightarrow S \neq (0)$ be a ring homomorphism. $\ker f$ is an ideal of R , and it can be either (0) or (1) as per hypothesis. But $\ker f \neq R$ since we at least have $1_R \notin \ker f$ by definition. Hence, $\ker f = (0)$, which implies f is injective³.

³Recall from the first course in algebra: A ring homomorphism is injective iff its kernel is (0) .

- (3) \implies (1). Suppose every homomorphism of R to a non-zero ring is injective. We want to show that R is a field, i.e., every non-zero element is a unit. Suppose there is an element $x \in R$ which is not a unit. Then $(x) \neq (1)$ (because if it was (1) , then that would mean $y \cdot x = 1 \implies x$ is a unit).

Consider the canonical projection map $\pi : R \rightarrow R/(x)$ for which $\ker \pi = (x)$. Since $(x) \neq (1)$, i.e., since $(x) \neq R$, $R/(x) \neq (0)$. So, $\ker \pi = (0)$ by hypothesis, which implies $(x) = (0) \implies x = 0$. Hence, the only non-unit in R is 0, and so every non-zero element should be a unit.

□

4 References

References

- [AM69] Michael Francis Atiyah and Ian G. MacDonald. *Introduction to Commutative Algebra*. Addison-Wesley Publishing Company, 1969.
- [Eis95] David Eisenbud. *Commutative Algebra: with a View Toward Algebraic Geometry*. New York: Springer-Verlag, 1995. ISBN: 978-0387942681.